autocorres: translate accesses to nested structs correctly. See tests/proof-tests/nested_struct.thy.
This should (finally) close issue JIRA VER-321. Unfortunately it also breaks some other things,
such as heap_abs_syntax, which we'll need to examine later.

tools/autocorres/tests/examples/SchorrWaite.thy
@@ -54,12 +54,11 @@ begin
 declare fun_upd_apply[simp del]
 
 install_C_file "schorr_waite.c"
-
 autocorres [heap_abs_syntax] "schorr_waite.c"
 
 (* AutoCorres doesn't successfully recognize all boolean variables yet,
    so this saves us some typing *)
-abbreviation Cbool where "Cbool b \<equiv> if b then 1 else 0"
+abbreviation Cbool where "Cbool b \<equiv> if b then 1 else (0::int)"
 
 declare fun_upd_apply [simp]
 
@@ -374,9 +373,17 @@ abbreviation schorr_waite'_measure where
      let stack = (THE stack. schorr_waite'_inv s s0 R p t cond stack)
      in (card {x \<in> R. s[x]\<rightarrow>m = 0}, card {x \<in> set stack. s[x]\<rightarrow>c = 0}, length stack)"
 
+(* FIXME: heap_abs_syntax failure *)
+lemma syntax_hack_simp:
+  "heap_node_C_update (\<lambda>b. b(a := r_C_update (\<lambda>c. l_C (b a)) (b a))) s =
+     update_node_r s a (get_node_l s a)"
+  by (simp add: update_node_r_def get_node_l_def)
+
 schematic_lemma schorr_waite'_prove_def [standard]:
   "schorr_waite' root \<equiv> ?A root (s0 :: lifted_globals) (R :: node_C ptr set)"
   apply (subst schorr_waite'_def[abs_def])
+  apply (subst syntax_hack_simp[abs_def])
+  apply (subst ptr_coerce.simps)+
   apply (subst whileLoop_add_inv
            [where I = "\<lambda>(p, cond, t) s. \<exists>stack. schorr_waite'_inv s s0 R p t cond stack"
               and M = "(\<lambda>((p, cond, t), s). schorr_waite'_measure s s0 R p t cond)"])
@@ -429,7 +436,7 @@ proof (tactic "wp_all_tac @{context}",
   {
     fix s
     assume "?Pre root s"
-    thus "\<forall>x. (?inv NULL root (Cbool (root \<noteq> NULL \<and> s[root]\<rightarrow>m = 0)) s) \<and>
+    thus "\<forall>x. ?inv NULL root (Cbool (root \<noteq> NULL \<and> s[root]\<rightarrow>m = 0)) s \<and>
               (root \<noteq> NULL \<longrightarrow> is_valid_node_C s root)"
       by (auto simp: reachable_def addrs_def)
   next
